[comment]: render
#  Section 5.1 – Growth and Decay with Integral Exponents  
**Guided Notes**



##  I. Opening Exploration: How Do You Usually Calculate Growth?

###  Scenario:  
You buy a laptop for \$1000. The value increases by **5%** after one year.  
How much is it worth after one year?

### Method 1: Add the growth  
- Step 1: Find 5% of 1000 →  
  $0.05 \times 1000 = \underline{\hspace{2cm}}$

- Step 2: Add that to the original:  
  $1000 + \underline{\hspace{2cm}} = \underline{\hspace{3cm}}$



### Method 2: Multiply by $1 + 0.05$  
- Step 1: Write $1 + 0.05 = \underline{\hspace{2cm}}$

- Step 2: Multiply:  
  $1000 \times 1.05 = \underline{\hspace{3cm}}$

These methods give the same result… so why use the second one?



### Let’s Keep Going...

What if the laptop keeps increasing in value by 5% each year?

- After 2 years (Method 1):
  - Find 5% of Year 1 Value →  
    $0.05 \times \underline{\hspace{2cm}} = \underline{\hspace{3cm}}$  
  - Add: $\underline{\hspace{2cm}} + \underline{\hspace{2cm}} = \underline{\hspace{3cm}}$

- After 2 years (Method 2):  
  $1000 \times 1.05^2 = \underline{\hspace{3cm}}$



### Key Insight 

Using $(1 + r)^n$ makes it easier to apply **the same percent change** multiple times.  
This is the foundation of **exponential growth** and **decay**.

> Exponential Growth Formula:  
> $A = A_0(1 + r)^n$

> Exponential Decay Formula:  
> $A = A_0(1 - r)^n$

Where:  
- $A_0$ = starting amount  
- $r$ = growth or decay rate (as a decimal)  
- $n$ = number of time periods



##  II. Rules of Exponents

Fill in the rule, then write a short explanation or justification of why the rule works.



### 1. Product Rule:  
If $a^m \cdot a^n = \underline{\hspace{3cm}}$

**Why does this rule work?**  
> ________________________________________________________________



### 2. Quotient Rule:  
If $\dfrac{a^m}{a^n} = \underline{\hspace{3cm}}$

**Why does this rule work?**  
> ________________________________________________________________



### 3. Power of a Power Rule:  
If $(a^m)^n = \underline{\hspace{3cm}}$

**Why does this rule work?**  
> ________________________________________________________________



### 4. Power of a Product Rule:  
If $(ab)^n = \underline{\hspace{3cm}}$

**Why does this rule work?**
> ________________________________________________________________



### 5. Zero Exponent Rule:  
If $a^0 = \underline{\hspace{3cm}}$ (where $a \ne 0$)

**Why does this rule work?**  
> ________________________________________________________________



### 6. Negative Exponent Rule:  
If $a^{-n} = \underline{\hspace{3cm}}$ (where $a \ne 0$)

**Why does this rule work?**  
> ________________________________________________________________



##  III. Practice: Simplifying with Exponents

Simplify each expression completely. Show all steps.

###  A. With Numbers Only

1. $\left( \dfrac{2^3}{2^5} \right) = \underline{\hspace{5cm}}$

2. $(3^{-1} + 4^{-1})^{-1} = \underline{\hspace{5cm}}$

3. $\left(\dfrac{5^{-2} \cdot 10^3}{2^{-1} \cdot 5}\right) = \underline{\hspace{5cm}}$

4. $(2^{-3})^4 = \underline{\hspace{5cm}}$

5. $\dfrac{6^0 + 2^{-1}}{3^{-2}} = \underline{\hspace{5cm}}$



###  B. With Variables

6. $\dfrac{x^5 \cdot x^{-3}}{x^2} = \underline{\hspace{5cm}}$

7. $\left(\dfrac{a^4b^{-2}}{a^{-1}b^3}\right)^2 = \underline{\hspace{5cm}}$

8. $\dfrac{(m^{-3}n^2)^2}{n^{-4}m} = \underline{\hspace{5cm}}$

9. $x^{-1} + y^{-1} = \dfrac{1}{x} + \dfrac{1}{y} = \underline{\hspace{5cm}}$

10. $\left( \dfrac{1}{x^{-1} + y^{-1}} \right) = \underline{\hspace{5cm}}$


## IV. Reflection

- What’s the difference between a **negative exponent** and a **subtraction of exponents**?

> ________________________________________________________________

- When do you need to flip a fraction when simplifying exponents?

> ________________________________________________________________

- Why is exponential growth more powerful than adding a fixed amount each time?

> ________________________________________________________________


